Details for Hurd Monad (#8)
* monad laws

* naming

* format

Library/Model/Monad.dfy
@@ -1,7 +1,7 @@
 /*******************************************************************************
-*  Copyright by the contributors to the Dafny Project
-*  SPDX-License-Identifier: MIT
-*******************************************************************************/
+ *  Copyright by the contributors to the Dafny Project
+ *  SPDX-License-Identifier: MIT
+ *******************************************************************************/
 
 include "RandomNumberGenerator.dfy"
 include "MeasureTheory.dfy"
@@ -69,9 +69,66 @@ module Monad {
     Bind(m, (a: A) => Return(f(a)))
   }
 
+  function Join<A>(ff: Hurd<Hurd<A>>): Hurd<A> {
+    (s: RNG) =>
+      var (f, s') := ff(s);
+      f(s')
+  }
+
   /*******
    Lemmas  
   *******/
+
+  lemma UnitalityBindReturn<A,B>(a: A, g: A -> Hurd<B>, s: RNG)
+    ensures Bind(Return(a), g)(s) == g(a)(s)
+  {}
+
+  lemma BindIsAssociative<A,B,C>(f: Hurd<A>, g: A -> Hurd<B>, h: B -> Hurd<C>, s: RNG)
+    ensures Bind(Bind(f, g), h)(s) == Bind(f, (a: A) => Bind(g(a), h))(s)
+  {
+    var (a, s') := f(s);
+    var (a', s'') := g(a)(s');
+    assert (a', s'') == Bind(f, g)(s);
+    calc {
+      Bind(Bind(f, g), h)(s);
+      h(a')(s'');
+      Bind(g(a), h)(s');
+      Bind(f, (a: A) => Bind(g(a), h))(s);
+    }
+  }
+
+  lemma CompositionIsAssociative<A,B,C,D>(f: A -> Hurd<B>, g: B -> Hurd<C>, h: C -> Hurd<D>, a: A, s: RNG)
+    ensures Composition(Composition(f, g), h)(a)(s) == Composition(f, Composition(g, h))(a)(s)
+  {
+    BindIsAssociative(f(a), g, h, s);
+  }
+
+  lemma UnitalityJoinReturn<A>(f: Hurd<A>, s: RNG)
+    ensures Join(Map(Return, f))(s) == Join(Return(f))(s)
+  {
+    var (a, t) := f(s);
+    calc {
+      Join(Return(f))(s);
+    ==
+      (a, t);
+    ==
+      Join(Map(Return, f))(s);
+    }
+  }
+
+  lemma JoinIsAssociative<A>(fff: Hurd<Hurd<Hurd<A>>>, s: RNG)
+    ensures Join(Map(Join, fff))(s) == Join(Join(fff))(s)
+  {
+    var (ff, t) := fff(s);
+    var (f, u) := ff(t);
+    calc {
+      Join(Map(Join, fff))(s);
+    ==
+      f(u);
+    ==
+      Join(Join(fff))(s);
+    }
+  }
 
   lemma {:axiom} TailIsRNG(s: RNG)
     ensures IsRNG((n: nat) => s(n+1))
